@prefix : <http://linkedmultimedia.org/sparql-mm/1.0.0/ontology#> .
@prefix owl: <http://www.w3.org/2002/07/owl#> .
@prefix rdf: <http://www.w3.org/1999/02/22-rdf-syntax-ns#> .
@prefix xml: <http://www.w3.org/XML/1998/namespace> .
@prefix xsd: <http://www.w3.org/2001/XMLSchema#> .
@prefix rdfs: <http://www.w3.org/2000/01/rdf-schema#> .
@base <http://linkedmultimedia.org/sparql-mm/ns/1.0.0/ontology> .

<http://linkedmultimedia.org/sparql-mm/ns/1.0.0/ontology> rdf:type owl:Ontology .


#################################################################
#
#    Object Properties
#
#################################################################


###  http://linkedmultimedia.org/sparql-mm/ns/1.0.0/ontology#hasEndPoint

:hasEndPoint rdf:type owl:ObjectProperty ;
             
             rdfs:label "hasEndPoint" ;
             
             rdfs:comment "A shape has a two dimensional Vector as endpoint (e.g. a line)." ;
             
             rdfs:domain :Line ;
             
             rdfs:subPropertyOf :hasVector_2D .



###  http://linkedmultimedia.org/sparql-mm/ns/1.0.0/ontology#hasEndTime

:hasEndTime rdf:type owl:ObjectProperty ;
            
            rdfs:label "hasEndTime" ;
            
            rdfs:comment "A time class has a certain Time as endpoint." ;
            
            rdfs:domain :Interval ;
            
            rdfs:subPropertyOf :hasTime .



###  http://linkedmultimedia.org/sparql-mm/ns/1.0.0/ontology#hasHeight

:hasHeight rdf:type owl:ObjectProperty ;
           
           rdfs:label "hasHeight" ;
           
           rdfs:comment "A shape has a one dimensional vector as height (e.g. a rectangle)." ;
           
           rdfs:domain :Rectangle ;
           
           rdfs:subPropertyOf :hasVector_1D .



###  http://linkedmultimedia.org/sparql-mm/ns/1.0.0/ontology#hasRadius

:hasRadius rdf:type owl:ObjectProperty ;
           
           rdfs:label "hasRadius" ;
           
           rdfs:comment "A shape has a one dimensional vector as radius (e.g. a circle)." ;
           
           rdfs:domain :Circle ;
           
           rdfs:subPropertyOf :hasVector_1D .



###  http://linkedmultimedia.org/sparql-mm/ns/1.0.0/ontology#hasStartPoint

:hasStartPoint rdf:type owl:ObjectProperty ;
               
               rdfs:label "hasStartPoint" ;
               
               rdfs:comment "A shape has a two dimensional Vector as startpoint (e.g. a line)." ;
               
               rdfs:domain :Line ;
               
               rdfs:subPropertyOf :hasVector_2D .



###  http://linkedmultimedia.org/sparql-mm/ns/1.0.0/ontology#hasStartTime

:hasStartTime rdf:type owl:ObjectProperty ;
              
              rdfs:label "hasStartTime" ;
              
              rdfs:comment "A time class has a certain Time as startpoint." ;
              
              rdfs:domain :Interval ;
              
              rdfs:subPropertyOf :hasTime .



###  http://linkedmultimedia.org/sparql-mm/ns/1.0.0/ontology#hasTime

:hasTime rdf:type owl:ObjectProperty ;
         
         rdfs:label "hasTime" ;
         
         rdfs:comment "A time class has a certain Time." ;
         
         rdfs:domain :Instant ;
         
         rdfs:range :Time .



###  http://linkedmultimedia.org/sparql-mm/ns/1.0.0/ontology#hasVector

:hasVector rdf:type owl:ObjectProperty ;
           
           rdfs:label "hasVector" ;
           
           rdfs:comment "A superclass of any relation between Thing and Vector." ;
           
           rdfs:range :Vector .



###  http://linkedmultimedia.org/sparql-mm/ns/1.0.0/ontology#hasVector_1D

:hasVector_1D rdf:type owl:ObjectProperty ;
              
              rdfs:label "hasVector 1D" ;
              
              rdfs:comment "A supertype for any relation between Thing an one dimensional Vectors." ;
              
              rdfs:range :Vector_1D ;
              
              rdfs:subPropertyOf :hasVector .



###  http://linkedmultimedia.org/sparql-mm/ns/1.0.0/ontology#hasVector_2D

:hasVector_2D rdf:type owl:ObjectProperty ;
              
              rdfs:label "hasVector 2D" ;
              
              rdfs:comment "A supertype for any relation between Thing an two dimensional Vectors." ;
              
              rdfs:range :Vector_2D ;
              
              rdfs:subPropertyOf :hasVector .



###  http://linkedmultimedia.org/sparql-mm/ns/1.0.0/ontology#hasWidth

:hasWidth rdf:type owl:ObjectProperty ;
          
          rdfs:label "hasWidth" ;
          
          rdfs:comment "A shape has a one dimensional vector as width (e.g. a rectangle)." ;
          
          rdfs:domain :Rectangle ;
          
          rdfs:subPropertyOf :hasVector_1D .



###  http://linkedmultimedia.org/sparql-mm/ns/1.0.0/ontology#hasXY

:hasXY rdf:type owl:ObjectProperty ;
       
       rdfs:label "hasXY" ;
       
       rdfs:comment "A shape has a two dimensional Vector (e.g. center of a circle)." ;
       
       rdfs:domain :Circle ,
                   :Point ,
                   :Rectangle ;
       
       rdfs:subPropertyOf :hasVector_2D .





#################################################################
#
#    Classes
#
#################################################################


###  http://linkedmultimedia.org/sparql-mm/ns/1.0.0/ontology#Circle

:Circle rdf:type owl:Class ;
        
        rdfs:label "Circle" ;
        
        rdfs:subClassOf :Curved ;
        
        rdfs:comment "A circle is defined by a two dimensional vector (center) and a one dimensional vector (radius)." .



###  http://linkedmultimedia.org/sparql-mm/ns/1.0.0/ontology#Curved

:Curved rdf:type owl:Class ;
        
        rdfs:label "Curved" ;
        
        rdfs:subClassOf :Shape ;
        
        owl:disjointWith :Polygon ;
        
        rdfs:comment "A superclass for all curved shapes." .



###  http://linkedmultimedia.org/sparql-mm/ns/1.0.0/ontology#Instant

:Instant rdf:type owl:Class ;
         
         rdfs:label "Instant" ;
         
         rdfs:subClassOf :TemporalEntity ;
         
         owl:disjointWith :Interval ;
         
         rdfs:comment "An Instant is defined by a Time." .



###  http://linkedmultimedia.org/sparql-mm/ns/1.0.0/ontology#Interval

:Interval rdf:type owl:Class ;
          
          rdfs:label "Interval" ;
          
          rdfs:subClassOf :TemporalEntity ;
          
          rdfs:comment "An Interval is defined by 2 Times (start and end)." .



###  http://linkedmultimedia.org/sparql-mm/ns/1.0.0/ontology#Line

:Line rdf:type owl:Class ;
      
      rdfs:label "Line" ;
      
      rdfs:subClassOf :SpatialEntity ;
      
      rdfs:comment "A line is defined by 2 two dimensional vectors (start and endpoint)." .



###  http://linkedmultimedia.org/sparql-mm/ns/1.0.0/ontology#NPT

:NPT rdf:type owl:Class ;
     
     rdfs:label "NPT" ;
     
     rdfs:subClassOf :Time ;
     
     rdfs:comment "Normal Play Time (NPT) like described in: Real Time Streaming Protocol (RTSP). IETF RFC 2326, April 1998. Available at http://www.ietf.org/rfc/rfc2326.txt." .



###  http://linkedmultimedia.org/sparql-mm/ns/1.0.0/ontology#Point

:Point rdf:type owl:Class ;
       
       rdfs:label "Point" ;
       
       rdfs:subClassOf :SpatialEntity ;
       
       rdfs:comment "A Point is defined by 1 two dimensional vector." .



###  http://linkedmultimedia.org/sparql-mm/ns/1.0.0/ontology#Polygon

:Polygon rdf:type owl:Class ;
         
         rdfs:label "Polygon" ;
         
         rdfs:subClassOf :Shape ;
         
         rdfs:comment "A superclass for all polygonial shapes." .



###  http://linkedmultimedia.org/sparql-mm/ns/1.0.0/ontology#Rectangle

:Rectangle rdf:type owl:Class ;
           
           rdfs:label "Rectangle" ;
           
           rdfs:subClassOf :Polygon ;
           
           rdfs:comment "A Rectangle is defined by a two dimensional vector (left-upper point) and 2 one dimensional vectors (width and height)." .



###  http://linkedmultimedia.org/sparql-mm/ns/1.0.0/ontology#SMPTE

:SMPTE rdf:type owl:Class ;
       
       rdfs:label "SMPTE" ;
       
       rdfs:subClassOf :Time ;
       
       rdfs:comment "SMPTE RP 136 Time and Control Codes for 24, 25 or 30 Frame-Per-Second Motion-Picture Systems." .



###  http://linkedmultimedia.org/sparql-mm/ns/1.0.0/ontology#Shape

:Shape rdf:type owl:Class ;
       
       rdfs:label "Shape" ;
       
       rdfs:subClassOf :SpatialEntity ;
       
       rdfs:comment "A superclass for all shapes." .



###  http://linkedmultimedia.org/sparql-mm/ns/1.0.0/ontology#SpatialEntity

:SpatialEntity rdf:type owl:Class ;
               
               rdfs:label "Spatial Entity" ;
               
               rdfs:subClassOf :SpatialThing ;
               
               rdfs:comment "A superclass of any spatial entities like point, line, polygone, curcle, etc." .



###  http://linkedmultimedia.org/sparql-mm/ns/1.0.0/ontology#SpatialThing

:SpatialThing rdf:type owl:Class ;
              
              rdfs:label "Spatial Thing" ;
              
              rdfs:comment "A superclass for any spatial thing." .



###  http://linkedmultimedia.org/sparql-mm/ns/1.0.0/ontology#TemporalEntity

:TemporalEntity rdf:type owl:Class ;
                
                rdfs:label "Temporal Entity" ;
                
                rdfs:subClassOf :TemporalThing ;
                
                owl:disjointWith :Time ;
                
                rdfs:comment "A superclass of any the temporal entity like instant, interval, etc." ;
                
                owl:disjointUnionOf ( :Instant
                                      :Interval
                                    ) .



###  http://linkedmultimedia.org/sparql-mm/ns/1.0.0/ontology#TemporalThing

:TemporalThing rdf:type owl:Class ;
               
               rdfs:label "Temporal Thing" ;
               
               rdfs:comment "A superclass for any temporal thing." .



###  http://linkedmultimedia.org/sparql-mm/ns/1.0.0/ontology#Time

:Time rdf:type owl:Class ;
      
      rdfs:label "Time" ;
      
      rdfs:subClassOf :TemporalThing ;
      
      rdfs:comment "A superclass for any kind of time specification." .



###  http://linkedmultimedia.org/sparql-mm/ns/1.0.0/ontology#UTC

:UTC rdf:type owl:Class ;
     
     rdfs:label "UTC" ;
     
     rdfs:subClassOf :Time ;
     
     rdfs:comment "Coordinated Universal Time (UTC) like defined in: Real Time Streaming Protocol (RTSP). IETF RFC 2326, April 1998. Available at http://www.ietf.org/rfc/rfc2326.txt." .



###  http://linkedmultimedia.org/sparql-mm/ns/1.0.0/ontology#Vector

:Vector rdf:type owl:Class ;
        
        rdfs:label "Vector" ;
        
        rdfs:subClassOf :SpatialThing ;
        
        rdfs:comment "A superclass for vectors." .



###  http://linkedmultimedia.org/sparql-mm/ns/1.0.0/ontology#Vector_1D

:Vector_1D rdf:type owl:Class ;
           
           rdfs:label "Vector 1D" ;
           
           rdfs:subClassOf :Vector ;
           
           rdfs:comment "A one dimensional vector." .



###  http://linkedmultimedia.org/sparql-mm/ns/1.0.0/ontology#Vector_2D

:Vector_2D rdf:type owl:Class ;
           
           rdfs:label "Vector 2D" ;
           
           rdfs:subClassOf :Vector ;
           
           rdfs:comment "A two dimensional vector." .





#################################################################
#
#    General axioms
#
#################################################################


[ rdf:type owl:AllDisjointClasses ;
  owl:members ( :Line
                :Point
                :Shape
              )
] .
[ rdf:type owl:AllDisjointClasses ;
  owl:members ( :NPT
                :SMPTE
                :UTC
              )
] .




###  Generated by the OWL API (version 3.5.0) http://owlapi.sourceforge.net

