@prefix : <http://linkedmultimedia.org/sparql-mm/1.0.0/ontology#> .
@prefix owl: <http://www.w3.org/2002/07/owl#> .
@prefix rdf: <http://www.w3.org/1999/02/22-rdf-syntax-ns#> .
@prefix xml: <http://www.w3.org/XML/1998/namespace> .
@prefix xsd: <http://www.w3.org/2001/XMLSchema#> .
@prefix rdfs: <http://www.w3.org/2000/01/rdf-schema#> .
@base <http://linkedmultimedia.org/sparql-mm/ns/2.0.0/ontology#> .

<http://linkedmultimedia.org/sparql-mm/ns/2.0.0/ontology#> rdf:type owl:Ontology .


#################################################################
#
#    Object Properties
#
#################################################################


###  http://linkedmultimedia.org/sparql-mm/ns/2.0.0/ontology#hasEndPoint

:hasEndPoint rdf:type owl:ObjectProperty ;

             rdfs:label "hasEndPoint" ;

             rdfs:comment "A shape has a two dimensional Vector as endpoint (e.g. a line)." ;

             rdfs:domain :Line ;

             rdfs:subPropertyOf :hasVector_2D .



###  http://linkedmultimedia.org/sparql-mm/ns/2.0.0/ontology#hasEndTime

:hasEndTime rdf:type owl:ObjectProperty ;

            rdfs:label "hasEndTime" ;

            rdfs:comment "A time class has a certain Time as endpoint." ;

            rdfs:domain :Interval ;

            rdfs:subPropertyOf :hasTime .



###  http://linkedmultimedia.org/sparql-mm/ns/2.0.0/ontology#hasHeight

:hasHeight rdf:type owl:ObjectProperty ;

           rdfs:label "hasHeight" ;

           rdfs:comment "A shape has a one dimensional vector as height (e.g. a rectangle)." ;

           rdfs:domain :Rectangle ;

           rdfs:subPropertyOf :hasVector_1D .



###  http://linkedmultimedia.org/sparql-mm/ns/2.0.0/ontology#hasRadius

:hasRadius rdf:type owl:ObjectProperty ;

           rdfs:label "hasRadius" ;

           rdfs:comment "A shape has a one dimensional vector as radius (e.g. a circle)." ;

           rdfs:domain :Circle ;

           rdfs:subPropertyOf :hasVector_1D .



###  http://linkedmultimedia.org/sparql-mm/ns/2.0.0/ontology#hasStartPoint

:hasStartPoint rdf:type owl:ObjectProperty ;

               rdfs:label "hasStartPoint" ;

               rdfs:comment "A shape has a two dimensional Vector as startpoint (e.g. a line)." ;

               rdfs:domain :Line ;

               rdfs:subPropertyOf :hasVector_2D .



###  http://linkedmultimedia.org/sparql-mm/ns/2.0.0/ontology#hasStartTime

:hasStartTime rdf:type owl:ObjectProperty ;

              rdfs:label "hasStartTime" ;

              rdfs:comment "A time class has a certain Time as startpoint." ;

              rdfs:domain :Interval ;

              rdfs:subPropertyOf :hasTime .



###  http://linkedmultimedia.org/sparql-mm/ns/2.0.0/ontology#hasTime

:hasTime rdf:type owl:ObjectProperty ;

         rdfs:label "hasTime" ;

         rdfs:comment "A time class has a certain Time." ;

         rdfs:domain :Instant ;

         rdfs:range :Time .



###  http://linkedmultimedia.org/sparql-mm/ns/2.0.0/ontology#hasVector

:hasVector rdf:type owl:ObjectProperty ;

           rdfs:label "hasVector" ;

           rdfs:comment "A superclass of any relation between Thing and Vector." ;

           rdfs:range :Vector .



###  http://linkedmultimedia.org/sparql-mm/ns/2.0.0/ontology#hasVector_1D

:hasVector_1D rdf:type owl:ObjectProperty ;

              rdfs:label "hasVector 1D" ;

              rdfs:comment "A supertype for any relation between Thing an one dimensional Vectors." ;

              rdfs:range :Vector_1D ;

              rdfs:subPropertyOf :hasVector .



###  http://linkedmultimedia.org/sparql-mm/ns/2.0.0/ontology#hasVector_2D

:hasVector_2D rdf:type owl:ObjectProperty ;

              rdfs:label "hasVector 2D" ;

              rdfs:comment "A supertype for any relation between Thing an two dimensional Vectors." ;

              rdfs:range :Vector_2D ;

              rdfs:subPropertyOf :hasVector .



###  http://linkedmultimedia.org/sparql-mm/ns/2.0.0/ontology#hasWidth

:hasWidth rdf:type owl:ObjectProperty ;

          rdfs:label "hasWidth" ;

          rdfs:comment "A shape has a one dimensional vector as width (e.g. a rectangle)." ;

          rdfs:domain :Rectangle ;

          rdfs:subPropertyOf :hasVector_1D .



###  http://linkedmultimedia.org/sparql-mm/ns/2.0.0/ontology#hasXY

:hasXY rdf:type owl:ObjectProperty ;

       rdfs:label "hasXY" ;

       rdfs:comment "A shape has a two dimensional Vector (e.g. center of a circle)." ;

       rdfs:domain :Circle ,
                   :Point ,
                   :Rectangle ;

       rdfs:subPropertyOf :hasVector_2D .


###  http://linkedmultimedia.org/sparql-mm/ns/2.0.0/ontology#hasSpatialEntity

:hasSpatialEntity rdf:type owl:ObjectProperty ,

                           owl:FunctionalProperty ;

       rdfs:label "hasSpatialEntity" ;

       rdfs:comment "The functional relation between a spatio-temporal entity and a spatial entity" ;

       rdf:domain :SpatioTemporalEntity ;

       rdf:range :SpatialEntity .


###  http://linkedmultimedia.org/sparql-mm/ns/2.0.0/ontology#hasTemporalEntity

:hasTemporalEntity rdf:type owl:ObjectProperty ,

                            owl:FunctionalProperty ;

       rdfs:label "hasSpatialEntity" ;

       rdfs:comment "The functional relation between a spatio-temporal entity and a temporal entity" ;

       rdf:domain :SpatioTemporalEntity ;

       rdf:range :TemporalEntity .

### http://linkedmultimedia.org/sparql-mm/ns/2.0.0/ontology#animates

:animates rdf:type owl:ObjectProperty ,

                   owl:FunctionalProperty ;

         rdfs:label "animates" ;

         rdfs:comment "A property that links a :Animation to a :SpatialTemporalEntity." ;

         rdf:domain :Animation ;

         rdf:range :SpatialEntity .

#################################################################
#
#    Classes
#
#################################################################


###  http://linkedmultimedia.org/sparql-mm/ns/2.0.0/ontology#Circle

:Circle rdf:type owl:Class ;

        rdfs:label "Circle" ;

        rdfs:subClassOf :Curved ;

        rdfs:comment "A circle is defined by a two dimensional vector (center) and a one dimensional vector (radius)." .



###  http://linkedmultimedia.org/sparql-mm/ns/2.0.0/ontology#Curved

:Curved rdf:type owl:Class ;

        rdfs:label "Curved" ;

        rdfs:subClassOf :Shape ;

        owl:disjointWith :Polygon ;

        rdfs:comment "A superclass for all curved shapes." .



###  http://linkedmultimedia.org/sparql-mm/ns/2.0.0/ontology#Instant

:Instant rdf:type owl:Class ;

         rdfs:label "Instant" ;

         rdfs:subClassOf :TemporalEntity ;

         owl:disjointWith :Interval ;

         rdfs:comment "An Instant is defined by a Time." .



###  http://linkedmultimedia.org/sparql-mm/ns/2.0.0/ontology#Interval

:Interval rdf:type owl:Class ;

          rdfs:label "Interval" ;

          rdfs:subClassOf :TemporalEntity ;

          rdfs:comment "An Interval is defined by 2 Times (start and end)." .



###  http://linkedmultimedia.org/sparql-mm/ns/2.0.0/ontology#Line

:Line rdf:type owl:Class ;

      rdfs:label "Line" ;

      rdfs:subClassOf :SpatialEntity ;

      rdfs:comment "A line is defined by 2 two dimensional vectors (start and endpoint)." .



###  http://linkedmultimedia.org/sparql-mm/ns/2.0.0/ontology#NPT

:NPT rdf:type owl:Class ;

     rdfs:label "NPT" ;

     rdfs:subClassOf :Time ;

     rdfs:comment "Normal Play Time (NPT) like described in: Real Time Streaming Protocol (RTSP). IETF RFC 2326, April 1998. Available at http://www.ietf.org/rfc/rfc2326.txt." .



###  http://linkedmultimedia.org/sparql-mm/ns/2.0.0/ontology#Point

:Point rdf:type owl:Class ;

       rdfs:label "Point" ;

       rdfs:subClassOf :SpatialEntity ;

       rdfs:comment "A Point is defined by 1 two dimensional vector." .



###  http://linkedmultimedia.org/sparql-mm/ns/2.0.0/ontology#Polygon

:Polygon rdf:type owl:Class ;

         rdfs:label "Polygon" ;

         rdfs:subClassOf :Shape ;

         rdfs:comment "A superclass for all polygonial shapes." .



###  http://linkedmultimedia.org/sparql-mm/ns/2.0.0/ontology#Rectangle

:Rectangle rdf:type owl:Class ;

           rdfs:label "Rectangle" ;

           rdfs:subClassOf :Polygon ;

           rdfs:comment "A Rectangle is defined by a two dimensional vector (left-upper point) and 2 one dimensional vectors (width and height)." .



###  http://linkedmultimedia.org/sparql-mm/ns/2.0.0/ontology#SMPTE

:SMPTE rdf:type owl:Class ;

       rdfs:label "SMPTE" ;

       rdfs:subClassOf :Time ;

       rdfs:comment "SMPTE RP 136 Time and Control Codes for 24, 25 or 30 Frame-Per-Second Motion-Picture Systems." .



###  http://linkedmultimedia.org/sparql-mm/ns/2.0.0/ontology#Shape

:Shape rdf:type owl:Class ;

       rdfs:label "Shape" ;

       rdfs:subClassOf :SpatialEntity ;

       rdfs:comment "A superclass for all shapes." .



###  http://linkedmultimedia.org/sparql-mm/ns/2.0.0/ontology#SpatialEntity

:SpatialEntity rdf:type owl:Class ;

               rdfs:label "Spatial Entity" ;

               rdfs:subClassOf :SpatialThing ;

               owl:disjointWith :Time ;

               rdfs:comment "A superclass of any spatial entities like point, line, polygone, curcle, etc." .



###  http://linkedmultimedia.org/sparql-mm/ns/2.0.0/ontology#SpatialThing

:SpatialThing rdf:type owl:Class ;

              rdfs:label "Spatial Thing" ;

              rdfs:comment "A superclass for any spatial thing." .



###  http://linkedmultimedia.org/sparql-mm/ns/2.0.0/ontology#TemporalEntity

:TemporalEntity rdf:type owl:Class ;

                rdfs:label "Temporal Entity" ;

                rdfs:subClassOf :TemporalThing ;

                owl:disjointWith :Time ;

                rdfs:comment "A superclass of any the temporal entity like instant, interval, etc." ;

                owl:disjointUnionOf ( :Instant
                                      :Interval
                                    ) .



###  http://linkedmultimedia.org/sparql-mm/ns/2.0.0/ontology#TemporalThing

:TemporalThing rdf:type owl:Class ;

               rdfs:label "Temporal Thing" ;

               rdfs:comment "A superclass for any temporal thing." .

### http://linkedmultimedia.org/sparql-mm/ns/2.0.0/ontology#Animation

:Animation rdf:type owl:Class ;

  rdfs:label "Animation" ;

  rdfs:comment "A superclass for all animations." .

###  http://linkedmultimedia.org/sparql-mm/ns/2.0.0/ontology#SpatioTemporalEntity
:SpatioTemporalEntity rdf:type owl:Class ;

               rdfs:label "Spatio-Temporal Entity" ;

               rdfs:comment "A class that relates to spatial and temporal features" ;

               rdfs:subClassOf
                [ a owl:Restriction ;
                  owl:onProperty :hasSpatialEntity ;
                  owl:cardinality "1"^^xsd:integer
                ] ,
                [ a owl:Restriction ;
                  owl:onProperty :hasTemporalEntity ;
                  owl:cardinality "1"^^xsd:integer
                ] .

###  http://linkedmultimedia.org/sparql-mm/ns/2.0.0/ontology#Time

:Time rdf:type owl:Class ;

      rdfs:label "Time" ;

      rdfs:subClassOf :TemporalThing ;

      rdfs:comment "A superclass for any kind of time specification." .



###  http://linkedmultimedia.org/sparql-mm/ns/2.0.0/ontology#UTC

:UTC rdf:type owl:Class ;

     rdfs:label "UTC" ;

     rdfs:subClassOf :Time ;

     rdfs:comment "Coordinated Universal Time (UTC) like defined in: Real Time Streaming Protocol (RTSP). IETF RFC 2326, April 1998. Available at http://www.ietf.org/rfc/rfc2326.txt." .



###  http://linkedmultimedia.org/sparql-mm/ns/2.0.0/ontology#Vector

:Vector rdf:type owl:Class ;

        rdfs:label "Vector" ;

        rdfs:subClassOf :SpatialThing ;

        rdfs:comment "A superclass for vectors." .



###  http://linkedmultimedia.org/sparql-mm/ns/2.0.0/ontology#Vector_1D

:Vector_1D rdf:type owl:Class ;

           rdfs:label "Vector 1D" ;

           rdfs:subClassOf :Vector ;

           rdfs:comment "A one dimensional vector." .



###  http://linkedmultimedia.org/sparql-mm/ns/2.0.0/ontology#Vector_2D

:Vector_2D rdf:type owl:Class ;

           rdfs:label "Vector 2D" ;

           rdfs:subClassOf :Vector ;

           rdfs:comment "A two dimensional vector." .





#################################################################
#
#    General axioms
#
#################################################################


[ rdf:type owl:AllDisjointClasses ;
  owl:members ( :Line
                :Point
                :Shape
              )
] .
[ rdf:type owl:AllDisjointClasses ;
  owl:members ( :NPT
                :SMPTE
                :UTC
              )
] .




###  Generated by the OWL API (version 3.5.0) http://owlapi.sourceforge.net
